Redefined paths

BinaryRelations.v
@@ -3,54 +3,8 @@ Require Import Coq.Relations.Relation_Operators.
 Require Import Coq.Lists.List.
 
 Require Import Setoid.
+Require Import Psatz.
 Require Import Tactics.General.
-
-Definition rel_singleton {A} (x y : A): relation A :=
-  fun x' y' => x' = x /\ y' = y -> True.
-
-(* This definition of reflexive transitive closure for the convenient inductive structure *)
-(* Notation "R ^*" := (clos_refl_trans_n1 _ R) (at level 35, format "R ^*"). *)
-Notation "R ^*" := (clos_refl_trans_n1 _ R) (at level 5, format "R ^*").
-
-Lemma rtc_trans {A}: forall R: relation A,
-  transitive A R^*.
-Proof.
-  intros R x y z Hxy Hyz.
-  induction Hyz.
-  - assumption.
-  - econstructor; eassumption.
-Qed.
-
-Lemma rtc_alt_trans {A}: forall (R: relation A) a b c,
-  R a b -> R^* b c -> R^* a c.
-Proof.
-  intros R a b c Hab Hbc.
-  eapply rtc_trans; [|eassumption].
-  econstructor.
-  - eassumption.
-  - constructor.
-Qed.
-
-Add Parametric Relation (A: Type) (R: relation A): A (clos_refl_trans_n1 A R)
-  reflexivity  proved by (rtn1_refl A R)
-  transitivity proved by (rtc_trans R)
-  as rtc_rel.
-
-
-Lemma rtc_1n_n1_equiv {A}: forall (R: relation A) a b,
-  clos_refl_trans_1n _ R a b <-> R^* a b.
-Proof.
-  (* intros R a b H1n.
-  induction H1n.
-  - constructor.
-  - induction IHH1n.
-    + econstructor.
-      * eassumption.
-      * constructor.
-    + econstructor.
-      * eassumption.
-      * apply IHIHH1n. *)
-Admitted.
 
 Definition is_serial {A} (R: relation A) := forall a, exists b, R a b.
 Definition serial A := {R: relation A | is_serial R}.
@@ -60,16 +14,279 @@ Definition serial A := {R: relation A | is_serial R}.
 Definition serial_witness {A} (R: relation A) := forall a, {b | R a b}.
 Definition serialT A := {R: relation A & serial_witness R}.
 
-Definition reachable {A} (R: relation A) (l: list A) (b: A) := exists a, In a l /\ R^* a b.
+Definition reachable {A} (R: relation A) (l: list A) (b: A) := 
+  exists a, In a l /\ clos_refl_trans_n1 A R a b.
 
-Definition is_serial_from {A} (R: relation A) s :=
-  forall s', R^* s s' -> exists s'', R s' s''.
+Definition is_serial_from {A} (R: relation A) s := forall s', 
+  clos_refl_trans A R s s' ->
+  exists s'', R s' s''.
 
-Definition serial_from_witness {A} (R: relation A) s :=
-  forall s', R^* s s' -> {s''| R s' s''}.
+Definition serial_from_witness {A} (R: relation A) s := forall s',
+  clos_refl_trans A R s s' ->
+  {s''| R s' s''}.
 
 Inductive steps : nat -> forall {A}, relation A -> relation A :=
   | steps_one   : forall {A} (R: relation A) x y,
       R x y -> steps 1 R x y
   | steps_multi : forall {A} n (R: relation A) x y z,
       steps n R x y -> R y x -> steps (S n) R x z.
+
+Definition rel_singleton {A} (x y : A): relation A :=
+  fun x' y' => x' = x /\ y' = y -> True.
+
+
+Definition relationT A := A -> A -> Type.
+
+Reserved Notation "R ^*" (at level 5, format "R ^*").
+Inductive rtcT {A} (R: relation A) x : A -> Type :=
+  | rtcT_refl :
+      R^* x x
+  | rtcT_step : forall y z,
+      R y z ->
+      R^* x y ->
+      R^* x z
+  where "R ^*" := (rtcT R).
+
+Definition rtcT_singleton {state} {R: relation state} {x y} (r: R x y)
+  : R^* x y :=
+  rtcT_step R x x y r (rtcT_refl R x).
+
+(* Definition rtc_ind_struct
+  (A: Type) (R: relation A) x (P: forall x y, R^* x y -> Prop)
+  (p_refl: P x x (rtn1_refl A R x))
+  (p_step: forall y z (Ryz: R y z) (Rxy: R^* x y),
+    P x y Rxy -> P x z (rtn1_trans A R x y z Ryz Rxy)) :=
+  fix F z (Rxy: R^* x z) : P x z Rxy :=
+    match Rxy with
+    | rtn1_refl _ _ _ => p_refl
+    | rtn1_trans _ _ _ y z0 Ryz Rxy => p_step y z0 Ryz Rxy (F y Rxy)
+    end.
+ *)
+(* Definition rtc_ind_struct
+  (A: Type) (R: relation A) (P: forall x y, R^* x y -> Prop)
+  (p_refl: forall x, P x x (rtn1_refl A R x))
+  (p_step: forall x y z (Ryz: R y z) (Rxy: R^* x y),
+    P x y Rxy -> P x z (rtn1_trans A R x y z Ryz Rxy)) :=
+  fix F x z (Rxy: R^* x z) : P x z Rxy :=
+    match Rxy with
+    | rtn1_refl _ _ _ => p_refl x
+    | rtn1_trans _ _ _ y z0 Ryz Rxy => p_step x y z0 Ryz Rxy (F x y Rxy)
+    end. *)
+
+Definition reflexiveT {A} (R: relationT A) := forall x, R x x.
+
+Definition symmetrycT {A} (R: relationT A) := forall x y,
+  R x y ->
+  R y x.
+
+Definition transitiveT {A} (R: relationT A) := forall x y z,
+  R x y ->
+  R y z -> 
+  R x z.
+
+Lemma rtcT_trans {A}: forall R: relation A,
+  transitiveT R^*.
+Proof.
+  intros R x y z Hxy Hyz.
+  induction Hyz.
+  - assumption.
+  - econstructor; eassumption.
+Defined.
+
+Lemma rtcT_step_rev {A}: forall (R: relation A) a b c,
+  R a b ->
+  R^* b c ->
+  R^* a c.
+Proof.
+  intros R a b c Hab Hbc.
+  eapply rtcT_trans; [|eassumption].
+  econstructor.
+  - eassumption.
+  - constructor.
+Defined.
+
+Inductive in_rtcT {A} {R: relation A} {a}
+  : forall {a'}, A -> R^* a a' -> Prop :=
+  | in_rtcT_head_refl :
+      in_rtcT a (rtcT_refl R a)
+  | in_rtcT_head_step : forall x x' r p,
+      in_rtcT x' (rtcT_step R a x x' r p)
+  | in_rtcT_tail : forall x x' y r p,
+      in_rtcT y p ->
+      in_rtcT y (rtcT_step R a x x' r p).
+
+(* indexed rtc *)
+
+Reserved Notation "R ^#" (at level 5, format "R ^#").
+Inductive rtcT_idx {A} (R: relation A) : nat -> A -> A -> Type :=
+  | rtcT_idx_refl : forall x,
+      R^#0 x x
+  | rtcT_idx_step : forall n x y z,
+      R y z ->
+      R^#n x y ->
+      R^#(S n) x z
+  where "R ^#" := (rtcT_idx R).
+
+Definition rtcT_idx_singleton {state} {R: relation state} {x y} (r: R x y)
+  : R^# 1 x y :=
+  rtcT_idx_step R 0 x x y r (rtcT_idx_refl R x).
+
+Theorem rtcT_idx_step_rev {state}: forall (R: relation state) n s s' x,
+  R s s' ->
+  R^# n s' x ->
+  R^# (S n) s x.
+Proof using.
+  intros R n s s' x Hstep Hpath.
+  induction Hpath.
+  - apply rtcT_idx_singleton.
+    assumption.
+  - econstructor.
+    + eassumption.
+    + applyc IHHpath.
+      assumption.
+Qed.
+
+(* Definition rtc_idx_ind_struct
+  (A: Type) (R: relation A) (P: forall n x y, R^# n x y -> Prop)
+  (p_refl: forall x, P 0 x x (rtc_idx_refl R x))
+  (p_step: forall n x y z (Ryz: R y z) (Rxy: R^# n x y),
+    P n x y Rxy -> P (S n) x z (rtc_idx_step R n x y z Ryz Rxy)) :=
+  fix F n x z (Rxy: R^# n x z) : P n x z Rxy :=
+    match Rxy as Rxy0 in (_^# n0 x0 y0) return (P n0 x0 y0 Rxy0) with
+    | rtc_idx_refl _ x0 => p_refl x0
+    | rtc_idx_step _ n0 x0 y z0 Ryz Rxy => p_step n0 x0 y z0 Ryz Rxy (F n0 x0 y Rxy)
+    end. *)
+
+(* Definition rtc_idx_ind_struct_fixed_origin
+  (A: Type) (R: relation A) x (P: forall n x y, R^# n x y -> Prop)
+  (p_refl: P 0 x x (rtc_idx_refl R x))
+  (p_step: forall n y z (Ryz: R y z) (Rxy: R^# n x y),
+    P n x y Rxy -> P (S n) x z (rtc_idx_step R n x y z Ryz Rxy)) :=
+  fix F n z (Rxy: R^# n x z) : P n x z Rxy :=
+    (* match Rxy as Rxy0 in (_^# n0 x0 y0) return (P n0 x0 y0 Rxy0) with *)
+    match Rxy with
+    | rtc_idx_refl _ x0 => p_refl
+    | rtc_idx_step _ n0 x0 y z0 Ryz Rxy => p_step n0 x0 y z0 Ryz Rxy (F n0 y Rxy)
+    end. *)
+
+(* (almost) transitivity *)
+Theorem rtcT_idx_combine {A}: forall n m (R: relation A) x y z,
+  R^# n x y ->
+  R^# m y z ->
+  R^# (n+m) x z.
+Proof using.
+  intros n m R x y z Hxy Hyz; revert x Hxy.
+  (* induction Hyz using rtc_idx_ind_struct; intros. *)
+  induction Hyz; intros.
+  - rewrite PeanoNat.Nat.add_0_r.
+    assumption.
+  - rewrite PeanoNat.Nat.add_succ_r.
+    econstructor.
+    + eassumption.
+    + applyc IHHyz.
+      assumption.
+Defined.
+
+Theorem rtcT_idx_to_rtcT {A n} {R: relation A} {x y}:
+  R^# n x y ->
+  R^* x y.
+Proof using.
+  introv H.
+  induction H.
+  - constructor.
+  - econstructor; eassumption.
+Defined.
+
+Theorem rtcT_to_rtcT_idx {A} {R: relation A} {x y}:
+  R^* x y ->
+  {n & R^# n x y}.
+Proof using.
+  introv H.
+  induction H.
+  - eexists. constructor.
+  - destruct exists IHrtcT n.
+    exists (S n).
+    econstructor; eassumption.
+Defined.
+
+Inductive in_rtcT_idx_at {A} {R: relation A} {a}
+  : forall {n a'}, A -> nat -> R^# n a a' -> Prop :=
+  | in_rtcT_idx_at_head_refl :
+      in_rtcT_idx_at a 0 (rtcT_idx_refl R a)
+  | in_rtcT_idx_at_head_step : forall n x x' r p,
+      in_rtcT_idx_at x' n (rtcT_idx_step R n a x x' r p)
+  | in_rtcT_idx_at_tail : forall n m x x' y r p,
+      in_rtcT_idx_at y m p ->
+      in_rtcT_idx_at y m (rtcT_idx_step R n a x x' r p).
+
+Inductive in_rtcT_idx {A} {R: relation A} {a}
+  : forall {n a'}, A -> R^# n a a' -> Prop :=
+  | in_rtcT_idx_head_refl :
+      in_rtcT_idx a (rtcT_idx_refl R a)
+  | in_rtcT_idx_head_step : forall n x x' r p,
+      in_rtcT_idx x' (rtcT_idx_step R n a x x' r p)
+  | in_rtcT_idx_tail : forall n x x' y r p,
+      in_rtcT_idx y p ->
+      in_rtcT_idx y (rtcT_idx_step R n a x x' r p).
+
+Theorem in_rtcT_idx_at__in_rtcT_idx {A}:
+  forall (R: relation A) x a b n m (r: R^# n a b),
+    in_rtcT_idx_at x m r ->
+    in_rtcT_idx x r.
+Proof using.
+  introv H.
+  induction H; constructor.
+  assumption.
+Qed.
+
+Theorem in_rtcT_idx__in_rtcT_idx_at {A}:
+  forall (R: relation A) x a b n (r: R^# n a b),
+    in_rtcT_idx x r ->
+    exists m, m <= n /\ in_rtcT_idx_at x m r.
+Proof using.
+  introv H.
+  induction H.
+  - eexists.
+    split; [|constructor].
+    reflexivity.
+  - eexists.
+    split; [|constructor].
+    lia.
+  - destruct exists IHin_rtcT_idx m.
+    exists m.
+    destruct IHin_rtcT_idx.
+    split.
+    + lia.
+    + constructor.
+      assumption.
+Qed. 
+
+Require Import Coq.Program.Equality.
+Theorem in_rtcT__in_rtcT_idx {A}:
+  forall (R: relation A) x a b (r: R^* a b),
+    in_rtcT x r ->
+    exists n (r': R^# n a b), in_rtcT_idx x r'.
+Proof using.
+  introv.
+  dependent induction r; intros.
+  - repeat eexists. repeat constructor.
+Admitted.
+
+Theorem in_rtcT_idx__in_rtcT {A}:
+  forall (R: relation A) x n a b (r: R^# n a b),
+    in_rtcT_idx x r ->
+    in_rtcT x (rtcT_idx_to_rtcT r).
+Proof using.
+  introv H.
+  induction H. 
+  - constructor.
+  - constructor.
+  - simpl.
+    constructor.
+    assumption.
+Qed.
+
+Definition in_rtcT_idx_before {state} {R: relation state} {n s s'}
+  x i (r: R^# n s s') := 
+  exists j, j < i /\ in_rtcT_idx_at x i r.
+
