Ctl/Paths.v
@@ -5,266 +5,61 @@ Require Import BinaryRelations.
 Require Import Coq.Program.Equality.
 Require Import Tactics.General.
 
-Inductive rtc_len {A} {R: relation A} : nat -> forall {x y}, R^* x y -> Prop :=
-  | rtc_len_0 : forall x,
-      rtc_len 0 (rtn1_refl A R x)
-  | rtc_len_S : forall n x y z Ryz Rxy,
-      rtc_len n Rxy ->
-      rtc_len (S n) (rtn1_trans A R x y z Ryz Rxy).
+Definition path {state} (R: relation state) (n: nat) (s: state) :=
+  {s' & R^# n s s'}.
 
-(* This definition purposefully separates the sequence with the length so that the 
-   length can be discarded
- *)
-Definition indexed_rtc {A} (R: relation A) n x y :=
-  exists r: R^* x y, rtc_len n r.
-
-Notation "R ^#" := (indexed_rtc R) (at level 5, format "R ^#").
-
-Theorem indexed_rtc_refl {A}: forall (R: relation A) s,
-  R^# 0 s s.
+Theorem path_refl {state}: forall (R: relation state) s,
+  path R 0 s.
 Proof using.
   intros.
   eexists.
   constructor.
 Qed.
 
-Theorem indexed_rtc_step {A}: forall (R: relation A) s x x' n,
-  R x x' ->
-  R^# n s x ->
-  R^# (S n) s x'.
-Proof using.
-  intros R s x x' n Hstep Hsteps.
-  destruct exists Hsteps Rsx.
-  exists (rtn1_trans A R s x x' Hstep Rsx).
-  constructor.
-  assumption.
-Qed.
-
-(* Inspired by the TLC tactic of the same name
-https://github.com/charguer/tlc/blob/c6c9b344f36df70d600756fe20f2017730e48604/src/LibTactics.v#L1702
-  Likely much simpler, this tactic `intros` all the dependent hypotheses
-  (bound by a `forall`), then `intros` based on identifer list argument
- *)
-Tactic Notation "introv" :=
-  repeat match goal with 
-  (* Note, this only works because `intro x` fail for implications *)
-  | |- forall x, _ => intro x
-  end.
-
-Tactic Notation "introv" ident_list(il) :=
-  introv; intros il.
-
-Definition clos_refl_trans_n1_ind_double
-  (A: Type) (R: relation A) x (P: A -> A -> Prop)
-  (p_refl: P x x) 
-  (p_step: forall y z, R y z -> R^* x y -> P x y -> P x z) :=
-  fix F y (Rxy: R^* x y) : P x y :=
-  match Rxy with 
-  | rtn1_refl _ _ _ => p_refl
-  | rtn1_trans _ _ _ y z Ryz Rxy => p_step y z Ryz Rxy (F y Rxy)
-  end.
-
-(* Print clos_refl_trans_n1.
-Inductive clos_refl_trans_n1_T (A : Type) (R : relation A) (x : A) : A -> Type :=
-  | rtn1_refl : clos_refl_trans_n1_T A R x x
-  | rtn1_trans : forall y z : A,
-      R y z -> 
-      clos_refl_trans_n1_T A R x y ->
-      clos_refl_trans_n1_T A R x z. *)
-
-(* Inducts over steps rather than states *)
-(* Definition clos_refl_trans_n1_ind_struct 
-  (A: Type) (R: relation A) x (P: forall x y, R^* x y -> Prop)
-  (p_refl: P x x (rtn1_refl A R x)) 
-  (p_step: forall y z (Ryz: R y z) (Rxy: R^* x y), P x y Rxy ->
-    P x z (rtn1_trans A R x y z Ryz Rxy)) :=
-  fix F y (Rxy: R^* x y) : P x y Rxy :=
-  match Rxy with 
-  | rtn1_refl _ _ _ => p_refl 
-  | rtn1_trans _ _ _ y z Ryz Rxy => p_step y z Ryz Rxy (F y Rxy)
-  end. *)
-
-(* This is the definition Coq would have given a Type *)
-Definition clos_refl_trans_n1_ind_struct2 
-  (A: Type) (R: relation A) x (P: forall y, R^* x y -> Prop)
-  (p_refl: P x (rtn1_refl A R x)) 
-  (p_step: forall y z (Ryz: R y z) (Rxy: R^* x y), P y Rxy ->
-    P z (rtn1_trans A R x y z Ryz Rxy)) :=
-  fix F y (Rxy: R^* x y) : P y Rxy :=
-  match Rxy with 
-  | rtn1_refl _ _ _ => p_refl 
-  | rtn1_trans _ _ _ y z Ryz Rxy => p_step y z Ryz Rxy (F y Rxy)
-  end.
-
-
-Theorem rtc_len_refl_inv: forall n A R x,
-  rtc_len n (rtn1_refl A R x) ->
-  n = 0.
-Proof.
-  introv H.
-
-
-Theorem rtc_len_add {A}: forall n m (R: relation A) x y z,
-  forall Rxy: R^* x y,
-  forall Ryz: R^* y z,
-    rtc_len n Rxy ->
-    rtc_len m Ryz ->
-    rtc_len (n+m) (rtc_trans R x y z Rxy Ryz).
-Proof using.
-  introv Hxy Hyz.
-  revert Hxy z Ryz Hyz.
-  induction Rxy using clos_refl_trans_n1_ind_struct; intros.
-  - invc Hxy.
-    + admit.
-    + 
-  - induction Ryz using clos_refl_trans_n1_ind_struct.
-    + 
-
-  induction Rxy.
-  dependent induction Rxy. intros.
-  - 
-
-(* (almost) transitivity *)
-Theorem indexed_rtc_combine {A}: forall n m (R: relation A) x y z,
-  R^# n x y ->
-  R^# m y z ->
-  R^# (n+m) x z.
-Proof using.
-  intros n m R x y z Hxy Hyz.
-  destruct exists Hxy Rxy.
-  destruct exists Hyz Ryz.
-  exists (rtc_trans _ _ _ _ Rxy Ryz).
-  induction R.
-  constructor.
-
-intros path_xy path_yz; revert n x path_xy.
-induction path_yz; intros.
-+ rewrite PeanoNat.Nat.add_0_r. 
-  assumption.
-+ rewrite PeanoNat.Nat.add_succ_r.
-  eapply path_to_step.
-  * eassumption.
-  * applyc IHpath_yz.
-    assumption.
-Defined.
-
-Definition path {state} (R: relation state) (n: nat) (s: state) :=
-  exists s', path_to R n s s'.
-
-Theorem path_refl {state}: forall (R: relation state) s,
-  path R 0 s.
-Proof using.
-  intros.
-  econstructor.
-  constructor.
-Qed.
-
 Theorem path_step {state}: forall (R: relation state) n s x x',
   R x x' ->
-  path_to R n s x ->
+  R^# n s x ->
   path R (S n) s.
 Proof using.
   intros.
-  econstructor.
+  eexists.
   econstructor; eassumption.
 Qed.
 
-Definition path_from_path_to {state} {R: relation state} {n s s'}
-  (p: path_to R n s s') : path R n s :=
-  ex_intro _ s' p.
-
-Inductive in_path_to_at {state} {R: relation state} {s}
-  : forall {s'}, state -> nat -> forall {n}, path_to R n s s' -> Prop :=
-  | in_path_to_at_head_refl :
-      in_path_to_at s 0 (path_to_refl s)
-  | in_path_to_at_head_step : forall x x' n r p,
-      in_path_to_at x' n (path_to_step s x x' n r p)
-  | in_path_to_at_tail : forall x x' y n m r p,
-      in_path_to_at y m p ->
-      in_path_to_at y m (path_to_step s x x' n r p).
+Definition rtcT_idx_to_path {state} {R: relation state} {n s s'}
+  (r: R^# n s s') : path R n s :=
+  existT _ s' r.
 
 Inductive in_path_at {state} {R: relation state} {n s} 
   : state -> nat -> path R n s -> Prop :=
-  | in_path_at_rule : forall x m s' (p: path_to R n s s'),
-      in_path_to_at x m p ->
-      in_path_at x m (path_from_path_to p).
-
-Inductive in_path_to {state} {R: relation state} {s}
-  : forall {s'}, state -> forall {n}, path_to R n s s' -> Prop :=
-  | in_path_to_head_refl :
-      in_path_to s (path_to_refl s)
-  | in_path_to_head_step : forall x x' n r p,
-      in_path_to x' (path_to_step s x x' n r p)
-  | in_path_to_tail : forall x x' y n r p,
-      in_path_to y p ->
-      in_path_to y (path_to_step s x x' n r p).
+  | in_path_at_rule : forall x m s' (r: R^# n s s'),
+      in_rtcT_idx_at x m r ->
+      in_path_at x m (rtcT_idx_to_path r).
 
 Inductive in_path {state} {R: relation state} {n s} 
   : state -> path R n s -> Prop :=
-  | in_path_rule : forall x s' (p: path_to R n s s'),
-      in_path_to x p ->
-      in_path x (path_from_path_to p).
+  | in_path_rule : forall x s' (r: R^# n s s'),
+      in_rtcT_idx x r ->
+      in_path x (rtcT_idx_to_path r).
 
-Theorem in_path_from_in_path_to {state}:
-  forall (R: relation state) n s s' (p: path_to R n s s') x,
-    in_path_to x p ->
-    in_path x (path_from_path_to p).
-Proof using.
-  intros.
-  destruct H; repeat constructor.
-  assumption.
-Qed. 
-
-Theorem in_path_at_from_in_path_to_at {state}:
-  forall (R: relation state) n s s' i (p: path_to R n s s') x,
-    in_path_to_at x i p ->
-    in_path_at x i (path_from_path_to p).
-Proof using.
-  intros.
-  destruct H; repeat constructor.
-  assumption.
-Qed. 
-
-Theorem in_path_to_impl_in_path_to_at {state} {R: relation state} {n s s'}:
-  forall x (p: path_to R n s s'), 
-    in_path_to x p ->
-    exists i, in_path_to_at x i p.
-Proof.
-  intros x p H.
-  induction H. 
-  - eexists; constructor.
-  - eexists; constructor.
-  - destruct exists IHin_path_to i.
-    eexists.
-    constructor.
-    eassumption.
-Qed.
-
-Theorem in_path_to_at_impl_in_path_to {state} {R: relation state} {n s s'}:
-  forall x i (p: path_to R n s s'),
-    in_path_to_at x i p ->
-    in_path_to x p.
-Proof.
-  intros x i p H.
-  induction H; constructor.
-  assumption.
-Qed.
-
-Theorem in_path_impl_in_path_at {state} {R: relation state} {n s}:
+Theorem in_path__in_path_at {state} {R: relation state} {n s}:
   forall x (p: path R n s), 
     in_path x p ->
-    exists i, in_path_at x i p.
+    exists m, m <= n /\ in_path_at x m p.
 Proof.
   intros x p H.
   invc H.
-  apply in_path_to_impl_in_path_to_at in H0.
-  destruct exists H0 i.
-  exists i.
-  constructor.
-  assumption.
+  apply in_rtcT_idx__in_rtcT_idx_at in H0.
+  destruct exists H0 m.
+  exists m.
+  destruct H0.
+  split.
+  - assumption.
+  - constructor.
+    assumption.
 Qed.
 
-Theorem in_path_at_impl_in_path {state} {R: relation state} {n s}:
+Theorem in_path_at__in_path {state} {R: relation state} {n s}:
   forall x i (p: path R n s),
     in_path_at x i p ->
     in_path x p.
@@ -272,42 +67,17 @@ Proof.
   intros x i p H.
   invc H.
   constructor.
-  eapply in_path_to_at_impl_in_path_to.
+  eapply in_rtcT_idx_at__in_rtcT_idx.
   eassumption.
 Qed.
-
-Definition in_path_to_before {state} {R: relation state} {n s s'}
-  x i (p: path_to R n s s') := 
-  exists j, j < i /\ in_path_to_at x i p.
 
 Definition in_path_before {state} {R: relation state} {n s} x i (p: path R n s) := 
   exists j, j < i /\ in_path_at x i p.
 
-
 (* A single-step path *)
-Definition path_to_singleton {state} {R: relation state} {x y} (r: R x y)
-  : path_to R 1 x y :=
-  path_to_step x x y 0 r (path_to_refl x).
-
 Definition path_singleton {state} {R: relation state} {x y} (r: R x y)
   : path R 1 x :=
-  path_from_path_to (path_to_singleton r).
-
-
-Theorem path_to_step_rev {state}: forall (R: relation state) n s s' x,
-  R s s' ->
-  path_to R n s' x ->
-  path_to R (S n) s x.
-Proof using.
-  intros R n s s' x Hstep Hpath.
-  induction Hpath.
-  - apply path_to_singleton.
-    assumption.
-  - econstructor.
-    + eassumption.
-    + applyc IHHpath.
-      assumption.
-Qed.
+  rtcT_idx_to_path (rtcT_idx_singleton r).
 
 Theorem path_step_rev {state}: forall (R: relation state) n s s',
   R s s' ->
@@ -316,169 +86,16 @@ Theorem path_step_rev {state}: forall (R: relation state) n s s',
 Proof using.
   intros R n s s' Hstep Hpath.
   destruct exists Hpath x.
-  eapply path_from_path_to.
-  eapply path_to_step_rev; eassumption.
+  eapply rtcT_idx_to_path.
+  eapply rtcT_idx_step_rev; eassumption.
 Qed.
 
-(*
-Require Import Psatz.
-Definition path_pop n {state} {R: relation state} {m s} (p: path R s m) 
-  : {s' & path R s' (m-n)}.
-  induction n.
-  - exists s.
-    replace (m - 0) with m by lia.
-    assumption.
-  - destruct exists IHn s'.
-    inv IHn.
-    + exists s'.
-      rewrite <- H1 in IHn.
-      replace (m - S n) with 0 by lia.
-      assumption.
-    + exists s'0.
-      replace (m - S n) with n0 by lia.
-      assumption.
-Qed.
-
-Definition path_tail {state} {R: relation state} {s n}
-  (p: path R s (S n)) : {s' & path R s' n}.
-inv p.
-eexists.
-eassumption.
-Defined.
-
-Lemma path_tail_correct {state} {R: relation state}:
-  forall s s' n r (p: path R s' n),
-  (* path_tail (path_step s s' n r p) = existT _ s' p. *)
-  projT2 (path_tail (path_step s s' n r p)) = p.
-Proof. reflexivity. Qed.
-
-Definition path_get_step {state} {R: relation state} {m s}
-  n (HinBounds: n < m) (p: path R s m) : {x & {y | R x y}}.
-move n at top.
-generalize_max.
-induction n; intros.
-- inv p.
-  + lia.
-  + repeat eexists. eassumption.
-- destruct m as [|m']; [lia|].
-  inv p.
-  clear H1.
-  assert (HLt: n < m') by lia.
-  specialize (IHn state R m' s' HLt X).
-  destruct exists IHn x y.
-  repeat eexists.
-  eapply IHn.
-Defined.
-
-Definition arbitrary_path {state} {R: relation state} 
-  (sw: serial_witness R) s n: path R s n.
-induction n.
-- constructor.
-- induction IHn.
-  + specialize (sw s).
-    destruct exists sw s'.
-    econstructor.
-    * eassumption.
-    * constructor.
-  + econstructor; eassumption.
-Defined.
-
-Definition gen_path {state} {R: relation state} {s}
-  (sfw: serial_from_witness R s) n: path R s n.
-induction n.
-- constructor.
-- induction IHn.
-  + specialize (sfw s (rtn1_refl _ R s)).
-    destruct exists sfw s'.
-    econstructor.
-    * eassumption.
-    * constructor.
-  + econstructor.
-    * eassumption.
-    * apply IHIHn.
-      intros s'' Hsteps.
-      apply sfw.
-      eapply rtc_alt_trans; eassumption.
-Defined.
-*)
-
-(*
-Theorem in_path_at_combine {state} {R: relation state}: 
-  forall n m i j x x' y y' s (p: path n R x x') (p': path m R y y'),
-    in_path_at y i p -> 
-    in_path_at s j p' -> 
-    (* Could also be path size (i+j) if we wanted to cut it as short as possible *)
-    (* exists p'': path (i+m) R x y', in_path_at s (i+j) p''. *)
-    exists l (p'': path l R x y'), in_path_at s (i+j) p''.
-Proof.
-  intros n m i j x x' y y' s p p' Hy Hs.
-  revert m j y' s p' Hs.
-  induction Hy; intros; try solve [eauto].
-  eapply path_step in p; [|eassumption]; clear r.
-  exists (S n + m) (path_combine p p').
-  induction Hs.
-  - simpl.
-  
-  (* Check (path_combine (path_step _ _ _ _ r p) p'). *)
-
-  (* intros s x i x' j n n' p p' Hx Hx'.
-  induction Hx; [eauto|eauto|].
-  specialize (IHHx p' Hx').
-  destruct exists IHHx n'' p''.
-  exists (S n'').
-  exists (path_step s s' n'' r p'').
-  constructor.
-  assumption.
-Qed. *)
-Admitted.
-*)
-
-(* 
-Theorem in_path_at_combine {state} {R: relation state}: 
-  forall s x i x' j n n' (p: path R s n) (p': path R x n'),
-    in_path_at x i p -> in_path_at x' j p' -> 
-    exists n'' (p'': path R s n''), in_path_at x' (i+j) p''.
-Proof.
-  intros s x i x' j n n' p p' Hx Hx'.
-  induction Hx; [eauto|eauto|].
-  specialize (IHHx p' Hx').
-  destruct exists IHHx n'' p''.
-  exists (S n'').
-  exists (path_step s s' n'' r p'').
-  constructor.
-  assumption.
-Qed. *)
-
-(* Theorem in_path_combine {state} {R: relation state}: 
-  forall s x x' n n' (p: path R s n) (p': path R x n'),
-    in_path x p -> in_path x' p' -> 
-    exists n'' (p'': path R s n''), in_path x' p''.
-Proof.
-  intros.
-  apply in_path_eq_in_path_at in H, H0.
-  destruct exists H i.
-  destruct exists H0 j.
-  eapply in_path_at_combine in H0; [|eassumption].
-  destruct exists H0 n'' p''.
-  exists n'' p''.
-  eapply in_path_at_to_in_path.
-  eassumption.
-Qed.  *)
-
-Theorem path_to_impl_rtc {state}: forall (R: relation state) n s s',
-  path_to R n s s' -> R^* s s'.
-Proof.
-  intros R n s s' H.
-  induction H.
-  - reflexivity.
-  - econstructor; eassumption.
-Qed.
-  
+(* This would require in_path be switched from `Prop` to `Type` *)
 Theorem in_path_impl_rtc {state}:
   forall (R: relation state) n s s' (p: path R n s),
     in_path s' p -> R^* s s'.
 Proof.
-  intros R n s s' p Hin.
+(* intros R n s s' p Hin.
   invc Hin.
   induction H.
   - constructor.
@@ -488,80 +105,62 @@ Proof.
       eassumption.
   - assumption.
 Qed.
+*)
+Abort.
 
-Lemma rtc_impl_path_to {state}: forall (R: relation state) s s',
-  R^* s s' -> exists n, path_to R n s s'.
+Theorem in_rtcT_idx_first {state}:
+  forall (R: relation state) n s s' (r: R^# n s s'),
+    in_rtcT_idx s r.
 Proof using.
-  intros R s s' H.
-  induction H.
-  - eexists. apply path_to_refl.
-  - destruct exists IHclos_refl_trans_n1 n.
-    exists (S n).
-    econstructor; eassumption.
+  intros.
+  induction r; constructor.
+  assumption. 
 Qed.
 
-
-Inductive in_rtc {state} {R: relation state} {s}
-  : forall {s'}, state -> R^* s s' -> Prop :=
-  | in_rtc_head_refl :
-      in_rtc s (rtn1_refl state R s)
-  | in_rtc_head_step : forall x x' r p,
-      in_rtc x' (rtn1_trans state R s x x' r p)
-  | in_rtc_tail : forall x x' y r p,
-      in_rtc y p ->
-      in_rtc y (rtn1_trans state R s x x' r p)
-  .
-
-Theorem in_path_to_impl_in_rtc {state}: forall (R: relation state) n s s' (p: path_to R n s s') x,
-  in_path_to x p ->
-  in_rtc x (path_to_impl_rtc R n s s' p).
+Theorem in_rtcT_idx_last {state}:
+  forall n (R: relation state) s s' (r: R^# n s s'),
+    in_rtcT_idx s' r.
 Proof using.
   intros.
-  induction H.
-Admitted.
+  destruct r; constructor.
+Qed.
 
-Check path_to_ind.
-Require Import Coq.Program.Equality.
-Theorem in_rtc_impl_in_path_to {state}: forall (R: relation state) n s s' (p: path_to R n s s') x,
-  in_rtc x (path_to_impl_rtc R n s s' p) ->
-  in_path_to x p.
+Theorem in_rtcT_idx__in_path {state}:
+  forall n (R: relation state) x s s' (r: R^# n s s'),
+    in_rtcT_idx x r ->
+    in_path x (rtcT_idx_to_path r).
 Proof using.
-  intros.
-  dependent induction H.
-
-
-Theorem in_path_to_first {state}:
-  forall (R: relation state) n s s' (p: path_to R n s s'),
-    in_path_to s p.
-Proof using.
-  intros.
-  elim p.
-  induction p.
-Admitted.
-
-Theorem in_path_to_last {state}:
-  forall n (R: relation state) s s' (p: path_to n R s s'),
-    in_path_to s' p.
-Proof using.
-  intros.
-  destruct p; constructor.
+  introv H.
+  destruct H; repeat constructor.
+  assumption.
 Qed.
 
 Theorem in_path_last {state}:
-  forall n (R: relation state) s s' (p: path_to n R s s'),
-    in_path s' (path_from_path_to p).
+  forall n (R: relation state) s s' (r: R^# n s s'),
+    in_path s' (rtcT_idx_to_path r).
 Proof using.
   intros.
-  eapply in_path_from_in_path_to.
-  apply in_path_to_last.
+  eapply in_rtcT_idx__in_path.
+  apply in_rtcT_idx_last.
 Qed.
 
-Lemma rtc_impl_in_some_path {state}: forall (R: relation state) s s',
-  R^* s s' -> exists n (p: path n R s), in_path s' p.
-Proof.
-  intros R s s' H.
-  apply rtc_impl_path_to in H.
-  destruct exists H n.
-  exists n.
-  exists (path_from_path_to H).
+Theorem in_path_first {state}:
+  forall n (R: relation state) s s' (r: R^# n s s'),
+    in_path s (rtcT_idx_to_path r).
+Proof using.
+  intros.
+  eapply in_rtcT_idx__in_path.
+  apply in_rtcT_idx_first.
+Qed.
+
+Lemma rtc__in_some_path {state}: forall (R: relation state) s s',
+  R^* s s' -> exists n (p: path R n s), in_path s' p.
+Proof using.
+  (* Why is this tactic intro-ing x? *)
+  (* introv. *)
+  intros R s s' r.
+  apply rtcT_to_rtcT_idx in r.
+  destruct exists r n.
+  exists n (rtcT_idx_to_path r).
+  apply in_path_last.
 Qed.
